Simu/Cor.v
@@ -83,14 +83,6 @@ Section SIMU.
   
   Hint Resolve expr_eval_simu Clight.assign_loc_value sem_cast_same.
   Hint Constructors compat_stmt state_context.
-
-  Remark ifte_translate:
-    forall (b: bool) s1 s2,
-      translate_stmt main_node (if b then s1 else s2) =
-      if b then (translate_stmt main_node s1) else (translate_stmt main_node s2).
-  Proof.
-    now destruct b.
-  Qed.
     
   Theorem simu:
     forall S1 S2,
